@prefix owl: <http://www.w3.org/2002/07/owl#> .
@prefix rdf: <http://www.w3.org/1999/02/22-rdf-syntax-ns#> .
@prefix xml: <http://www.w3.org/XML/1998/namespace> .
@prefix xsd: <http://www.w3.org/2001/XMLSchema#> .
@prefix rdfs: <http://www.w3.org/2000/01/rdf-schema#> .
@base <http://www.w3.org/2002/07/owl#> .

[ rdf:type owl:Ontology
 ] .

#################################################################
#    Object Properties
#################################################################

###  http://example.org/ontology#fromSatellite
<http://example.org/ontology#fromSatellite> rdf:type owl:ObjectProperty ;
                                            rdfs:domain <http://example.org/ontology#NTLImage> ;
                                            rdfs:range <https://www.eoknowledgehub.cn/eo/resource/satellite.2011-061A> ;
                                            rdfs:comment "Indicates which satellite captured the image."@en ;
                                            rdfs:label "from satellite"@en .


###  http://example.org/ontology#fromSensor
<http://example.org/ontology#fromSensor> rdf:type owl:ObjectProperty ;
                                         rdfs:domain <http://example.org/ontology#NTLImage> ;
                                         rdfs:range <https://www.eoknowledgehub.cn/eo/resource/sensor.1c58ddb9-2b4c-4fe0-9970-f5fdc7242f6b> ;
                                         rdfs:comment "Indicates which sensor (instrument) on the satellite captured the image."@en ;
                                         rdfs:label "from sensor"@en .


###  http://example.org/ontology#hasNTLImage
<http://example.org/ontology#hasNTLImage> rdf:type owl:ObjectProperty ;
                                          rdfs:domain <http://example.org/ontology#outageRecord> ;
                                          rdfs:range <http://example.org/ontology#NTLImage> ;
                                          rdfs:comment "Associates numerical outage record with NTL image from same day as recorded outage record."@en ;
                                          rdfs:label "has NTL image"@en .


###  http://example.org/ontology#hasOutageMap
<http://example.org/ontology#hasOutageMap> rdf:type owl:ObjectProperty ;
                                           rdfs:domain <http://example.org/ontology#NTLImage> ,
                                                       <http://example.org/ontology#OutageRecord> ;
                                           rdfs:range <http://example.org/ontology#OutageMap> ;
                                           rdfs:comment "Associates numerical NTL image or outage record with power outage severity map generated from NTL image."@en ;
                                           rdfs:label "has outage map"@en .


###  http://example.org/ontology#representsCounty
<http://example.org/ontology#representsCounty> rdf:type owl:ObjectProperty ;
                                               rdfs:domain <http://example.org/ontology#OutageRecord> ,
                                                           <http://www.w3.org/ns/ma-ont#Image> ;
                                               rdfs:range <https://dbpedia.org/ontology/AdministrativeRegion> ;
                                               rdfs:comment "Links an NTL image, outage map, or outage record to U.S. county (instance of dbo:AdministrativeRegion) that it depicts."@en ;
                                               rdfs:label "represents county"@en .


#################################################################
#    Data properties
#################################################################

###  http://example.org/ontology#numberOfOutages
<http://example.org/ontology#numberOfOutages> rdf:type owl:DatatypeProperty ;
                                              rdfs:domain <http://example.org/ontology#OutageRecord> ;
                                              rdfs:range xsd:integer ;
                                              rdfs:comment "Numerical outage record for county at date and time from Eagle-I dataset."@en ;
                                              rdfs:label "Number of Outages"@en .


###  http://example.org/ontology#recordDateTime
<http://example.org/ontology#recordDateTime> rdf:type owl:DatatypeProperty ;
                                             rdfs:domain <http://example.org/ontology#OutageRecord> ;
                                             rdfs:range xsd:dateTime ;
                                             rdfs:comment "Date and time for numerical outage record for county from Eagle-I dataset."@en ;
                                             rdfs:label "Outage Record DateTime"@en .


#################################################################
#    Classes
#################################################################

###  http://example.org/ontology#NTLImage
<http://example.org/ontology#NTLImage> rdf:type owl:Class ;
                                       rdfs:subClassOf <http://www.w3.org/ns/ma-ont#Image> ;
                                       rdfs:comment "A subclass of ma-ont:Image representing Nighttime Light images from Black Marble Dataset."@en ;
                                       rdfs:label "NTL Image"@en .


###  http://example.org/ontology#OutageMap
<http://example.org/ontology#OutageMap> rdf:type owl:Class ;
                                        rdfs:subClassOf <http://www.w3.org/ns/ma-ont#Image> ;
                                        rdfs:comment "Power outage map of county generated using NTL Imagery and Multimodal Outage Detector."@en ;
                                        rdfs:label "Outage Map"@en .


###  http://example.org/ontology#OutageRecord
<http://example.org/ontology#OutageRecord> rdf:type owl:Class ;
                                           rdfs:comment "Numerical outage record for county at date and time from Eagle-I dataset."@en ;
                                           rdfs:label "Outage Record"@en .


###  http://example.org/ontology#outageRecord
<http://example.org/ontology#outageRecord> rdf:type owl:Class .


###  http://www.w3.org/ns/ma-ont#Image
<http://www.w3.org/ns/ma-ont#Image> rdf:type owl:Class .


###  https://dbpedia.org/ontology/AdministrativeRegion
<https://dbpedia.org/ontology/AdministrativeRegion> rdf:type owl:Class .


###  https://www.eoknowledgehub.cn/eo/resource/satellite.2011-061A
<https://www.eoknowledgehub.cn/eo/resource/satellite.2011-061A> rdf:type owl:Class .


###  https://www.eoknowledgehub.cn/eo/resource/sensor.1c58ddb9-2b4c-4fe0-9970-f5fdc7242f6b
<https://www.eoknowledgehub.cn/eo/resource/sensor.1c58ddb9-2b4c-4fe0-9970-f5fdc7242f6b> rdf:type owl:Class .


###  Generated by the OWL API (version 5.1.18) https://github.com/owlcs/owlapi/
